lean/Lang/Interpreter.lean
@@ -24,20 +24,34 @@ abbrev Memory := @AList Loc (fun _ => Bool)
 def keySet {α : Type} {β : α → Type} (a : @AList α β) : Finset α :=
   Finset.mk (Multiset.ofList a.keys) a.nodupKeys
 
-/--
-Establishes a correspondance between the finite set of variables in the type
-checker and the association list in the interpreter.
--/
-lemma identEnvVars (h : typeCheckExpr (Expr.ident name) (keySet env)) : (AList.lookup name env).isSome := by
-  apply typeCheckExpr_ident at h
-  exact AList.lookup_isSome.mpr h
+/-- Given a proof that key ∈ assocList, lookups the key without fail. -/
+def AList.get [DecidableEq α] (key : α) (assocList : AList β) (h : key ∈ assocList) : β key :=
+  have isSome : (assocList.lookup key).isSome := by exact AList.lookup_isSome.mpr h
+
+  match assocList.lookup key, isSome with
+    | some v, _ => v
 
 /-- Evaluates an expression given a proof that the type checker has accepted this input. -/
 def evalExpr (expr : Expr) (env : Env) (mem : Memory) (h : typeCheckExpr expr (keySet env)) : Bool := match expr with
   | Expr.true => Bool.true
   | Expr.false => Bool.false
   | Expr.nand left right => !((evalExpr left env mem (typeCheckExpr_nandLeft h)) && (evalExpr right env mem (typeCheckExpr_nandRight h)))
-  | Expr.ident name => match AList.lookup name env, identEnvVars h with
-    | some p, _ => sorry -- TODO: we need proofs about memory
+  | Expr.ident name =>
+    let loc := AList.get name env (typeCheckExpr_ident h)
+    sorry -- TODO: retrieve from memory
+
+def evalStmt (stmt : Stmt) (env : Env) (mem : Memory) (h : typeCheckStmt stmt (keySet env)) : Env × Memory := match stmt with
+  | Stmt.decl name value =>
+    let v := evalExpr value env mem (typeCheckStmt_declValue h)
+    sorry -- TODO: store into memory
+  | Stmt.assign target value =>
+    let loc := AList.get target env (typeCheckStmt_assign h)
+    sorry -- TODO: store into memory
+  | Stmt.conditional condition body =>
+    let cond := evalExpr condition env mem (typeCheckStmt_conditionalCond h)
+    let (newEnv, newMem) := if cond then evalStmt body env mem (typeCheckStmt_conditionalBody h) else (env, mem)
+
+    -- we drop the new env, but keep the new mem
+    (env, newMem)
 
 -- def evalStmt (expr : Expr) (env : Env) (mem : Memory) (h : typeCheckExpr expr env) : Bool := match expr with
